pancake/pan_to_crepScript.sml
@@ -283,16 +283,21 @@ Definition compile_def:
          $ Dec (n+4) lc'
          $ crepLang$ExtCall f (n+1) (n+2) (n+3) (n+4)
      | _ => Skip) /\
-  (compile ctxt (ShMem op r ad) =
+  (compile ctxt (ShMemStore op r ad) =
+   (case (compile_exp ctxt r,compile_exp ctxt ad) of
+      ((e::_,_),(a::_, _)) =>
+        let n = FOLDR MAX 0 $ var_cexp e ++ var_cexp a
+        in
+          Dec (n+1) e $ ShMem (store_op op) (n+1) a
+    | _ => Skip)) ∧
+  (compile ctxt (ShMemLoad op r ad) =
    (case compile_exp ctxt ad of
       (a::_, _) =>
         (case FLOOKUP ctxt.vars r of
-           SOME (_, r'::_) => ShMem op r' a
-         | _ => Skip)
-    | _ => Skip)) ∧
+           SOME (_, r'::_) => ShMem (load_op op) r' a
+         | _ => Skip))) ∧
   (compile ctxt Tick = Tick)
 End
-
 
 Definition mk_ctxt_def:
   mk_ctxt vmap fs m (es:panLang$eid |-> 'a word) =
